

$$\frac{1}{(q; q^5)_\infty (q^4; q^5)_\infty} = \sum_{n=0}^{\infty} \frac{q^{n^2}}{(q; q)_n} \quad (1)$$

$$\frac{1}{(q; q^2)_\infty} = \sum_{n=0}^{\infty} \frac{q^{(n^2+n)/2}}{(q; q)_n} \quad (2)$$

$$\frac{(q^2; q^2)_\infty}{(q; q^2)_\infty} = \sum_{n=0}^{\infty} q^{(n^2+n)/2} \quad (3)$$

$$(q; q^1)_\infty = \sum_{n=0}^{\infty} \frac{(-1)^n q^{(n^2+n)/2}}{(q; q)_n} \quad (4)$$

$$\frac{(q^2; q^4)_\infty}{(q; q^4)_\infty (q^3; q^4)_\infty} = \sum_{n=0}^{\infty} \frac{q^{n^2}}{(q^2; q^2)_n} \quad (5)$$

$$(q; q^2)_\infty = \sum_{n=0}^{\infty} \frac{(-1)^n q^{n^2}}{(q^2; q^2)_n} \quad (6)$$

$$\begin{aligned} & \frac{1}{(q; q^{20})_\infty (q^3; q^{20})_\infty (q^4; q^{20})_\infty (q^5; q^{20})_\infty (q^7; q^{20})_\infty (q^9; q^{20})_\infty (q^{11}; q^{20})_\infty (q^{13}; q^{20})_\infty (q^{15}; q^{20})_\infty (q^{16}; q^{20})_\infty (q^{17}; q^{20})_\infty (q^{19}; q^{20})_\infty} \\ &= \sum_{n=0}^{\infty} \frac{q^{n^2}}{(q; q)_{2n}} \end{aligned} \quad (7)$$

$$\begin{aligned} & \frac{1}{(q; q^{20})_\infty (q^2; q^{20})_\infty (q^5; q^{20})_\infty (q^6; q^{20})_\infty (q^8; q^{20})_\infty (q^9; q^{20})_\infty (q^{11}; q^{20})_\infty (q^{12}; q^{20})_\infty (q^{14}; q^{20})_\infty (q^{15}; q^{20})_\infty (q^{18}; q^{20})_\infty (q^{19}; q^{20})_\infty} \\ &= \sum_{n=0}^{\infty} \frac{q^{n^2+n}}{(q; q)_{2n+1}} \end{aligned} \quad (8)$$

$$\frac{1}{(q; q^2)_\infty} = \sum_{n=0}^{\infty} \frac{q^{2n^2+n}}{(q; q)_{2n+1}} \quad (9)$$

$$\begin{aligned} & \frac{1}{(q; q^{16})_\infty (q^4; q^{16})_\infty (q^6; q^{16})_\infty (q^7; q^{16})_\infty (q^9; q^{16})_\infty (q^{10}; q^{16})_\infty (q^{12}; q^{16})_\infty (q^{15}; q^{16})_\infty} \\ &= \sum_{n=0}^{\infty} \frac{q^{2n^2+2n}}{(q; q)_{2n+1}} \end{aligned} \quad (10)$$

$$\begin{aligned} & \frac{1}{(q; q^{20})_\infty (q^3; q^{20})_\infty (q^5; q^{20})_\infty (q^7; q^{20})_\infty (q^8; q^{20})_\infty (q^9; q^{20})_\infty (q^{11}; q^{20})_\infty (q^{12}; q^{20})_\infty (q^{13}; q^{20})_\infty (q^{15}; q^{20})_\infty (q^{17}; q^{20})_\infty (q^{19}; q^{20})_\infty} \\ &= \sum_{n=0}^{\infty} \frac{q^{n^2+2n}}{(q; q)_{2n+1}} \end{aligned} \quad (11)$$

$$\frac{1}{(q; q^4)_\infty (q^2; q^4)_\infty (q^3; q^4)_\infty} = \sum_{n=0}^{\infty} \frac{q^{(n^2+n)/2} (-q; q)_n}{(q; q)_n} \quad (12)$$

$$\frac{1}{(q; q^2)_\infty} = \sum_{n=0}^{\infty} \frac{q^{(n^2+n)/2} (-q; q)_n}{(q^2; q^2)_n} \quad (13)$$

$$(q; q^1)_\infty = \sum_{n=0}^{\infty} \frac{(-1)^n q^{(n^2+n)/2} (-q; q)_n}{(q^2; q^2)_n} \quad (14)$$

$$\frac{1}{(q; q^5)_\infty (q^4; q^5)_\infty} = \sum_{n=0}^{\infty} \frac{q^{n^2} (-q; q)_n}{(q^2; q^2)_n} \quad (15)$$

$$\begin{aligned} & \frac{1}{(q; q^{14})_\infty (q^2; q^{14})_\infty (q^3; q^{14})_\infty (q^4; q^{14})_\infty (q^5; q^{14})_\infty (q^7; q^{14})_\infty (q^9; q^{14})_\infty (q^{10}; q^{14})_\infty (q^{11}; q^{14})_\infty (q^{12}; q^{14})_\infty (q^{13}; q^{14})_\infty} \\ &= \sum_{n=0}^{\infty} \frac{q^{n^2} (-q; q)_n}{(q; q)_{2n}} \end{aligned} \quad (16)$$

$$\frac{1}{(q; q^{14})_{\infty} (q^2; q^{14})_{\infty} (q^3; q^{14})_{\infty}^2 (q^4; q^{14})_{\infty} (q^5; q^{14})_{\infty} (q^7; q^{14})_{\infty} (q^9; q^{14})_{\infty} (q^{10}; q^{14})_{\infty} (q^{11}; q^{14})_{\infty}^2 (q^{12}; q^{14})_{\infty} (q^{13}; q^{14})_{\infty}} \\ = \sum_{n=0}^{\infty} \frac{q^{(n^2+n)/2} (-q; q)_n}{(q; q)_{2n}} \quad (17)$$

$$\frac{1}{(q; q^{10})_{\infty} (q^3; q^{10})_{\infty} (q^4; q^{10})_{\infty} (q^5; q^{10})_{\infty} (q^6; q^{10})_{\infty} (q^7; q^{10})_{\infty} (q^9; q^{10})_{\infty}} \\ = \sum_{n=0}^{\infty} \frac{q^{(3n^2+3n)/2} (-q; q)_n}{(q; q)_{2n+1}} \quad (18)$$

$$\frac{1}{(q; q^{14})_{\infty} (q^2; q^{14})_{\infty} (q^3; q^{14})_{\infty} (q^5; q^{14})_{\infty}^2 (q^6; q^{14})_{\infty} (q^7; q^{14})_{\infty} (q^8; q^{14})_{\infty} (q^9; q^{14})_{\infty}^2 (q^{11}; q^{14})_{\infty} (q^{12}; q^{14})_{\infty} (q^{13}; q^{14})_{\infty}} \\ = \sum_{n=0}^{\infty} \frac{q^{(n^2+3n)/2} (-q; q)_n}{(q; q)_{2n+1}} \quad (19)$$

$$\frac{1}{(q; q^{10})_{\infty} (q^2; q^{10})_{\infty} (q^3; q^{10})_{\infty} (q^5; q^{10})_{\infty} (q^7; q^{10})_{\infty} (q^8; q^{10})_{\infty} (q^9; q^{10})_{\infty}} \\ = \sum_{n=0}^{\infty} \frac{q^{(3n^2+n)/2} (-q; q)_n}{(q; q)_{2n+1}} \quad (20)$$

$$\frac{1}{(q; q^{14})_{\infty} (q^2; q^{14})_{\infty} (q^3; q^{14})_{\infty} (q^5; q^{14})_{\infty} (q^6; q^{14})_{\infty} (q^7; q^{14})_{\infty} (q^8; q^{14})_{\infty} (q^9; q^{14})_{\infty} (q^{11}; q^{14})_{\infty} (q^{12}; q^{14})_{\infty} (q^{13}; q^{14})_{\infty}} \\ = \sum_{n=0}^{\infty} \frac{q^{n^2+n} (-q; q)_n}{(q; q)_{2n+1}} \quad (21)$$

$$\frac{1}{(q; q^{14})_{\infty} (q^3; q^{14})_{\infty} (q^4; q^{14})_{\infty} (q^5; q^{14})_{\infty} (q^6; q^{14})_{\infty} (q^7; q^{14})_{\infty} (q^8; q^{14})_{\infty} (q^9; q^{14})_{\infty} (q^{10}; q^{14})_{\infty} (q^{11}; q^{14})_{\infty} (q^{13}; q^{14})_{\infty}} \\ = \sum_{n=0}^{\infty} \frac{q^{n^2+2n} (-q; q)_n}{(q; q)_{2n+1}} \quad (22)$$

$$\frac{1}{(q; q^8)_{\infty} (q^4; q^8)_{\infty} (q^7; q^8)_{\infty}} = \sum_{n=0}^{\infty} \frac{q^{n^2} (-q; q^2)_n}{(q^2; q^2)_n} \quad (23)$$

$$\frac{(q^6; q^{12})_{\infty}}{(q; q^{12})_{\infty} (q^2; q^{12})_{\infty} (q^3; q^{12})_{\infty} (q^4; q^{12})_{\infty} (q^5; q^{12})_{\infty} (q^7; q^{12})_{\infty} (q^8; q^{12})_{\infty} (q^9; q^{12})_{\infty} (q^{10}; q^{12})_{\infty} (q^{11}; q^{12})_{\infty}} \\ = \sum_{n=0}^{\infty} \frac{q^{n^2} (-q; q^2)_n}{(q; q)_{2n}} \quad (24)$$

$$\frac{1}{(q; q^4)_{\infty} (q^2; q^4)_{\infty} (q^3; q^4)_{\infty}} = \sum_{n=0}^{\infty} \frac{q^{n^2+n} (-q; q^2)_n}{(q; q)_{2n+1}} \quad (25)$$

$$\frac{1}{(q; q^{12})_{\infty} (q^3; q^{12})_{\infty} (q^4; q^{12})_{\infty} (q^5; q^{12})_{\infty} (q^6; q^{12})_{\infty} (q^7; q^{12})_{\infty} (q^8; q^{12})_{\infty} (q^9; q^{12})_{\infty} (q^{11}; q^{12})_{\infty}} \\ = \sum_{n=0}^{\infty} \frac{q^{n^2+2n} (-q; q^2)_n}{(q; q)_{2n+1}} \quad (26)$$

$$\frac{1}{(q; q^{12})_{\infty} (q^2; q^{12})_{\infty} (q^4; q^{12})_{\infty} (q^5; q^{12})_{\infty} (q^6; q^{12})_{\infty} (q^7; q^{12})_{\infty} (q^8; q^{12})_{\infty} (q^{10}; q^{12})_{\infty} (q^{11}; q^{12})_{\infty}} \\ = \sum_{n=0}^{\infty} \frac{q^{n^2+n} (-q^2; q^2)_n}{(q; q)_{2n+1}} \quad (27)$$

$$\frac{1}{(q; q^5)_{\infty} (q^4; q^5)_{\infty}} = \sum_{n=0}^{\infty} \frac{q^{n^2+n} (-q; q)_{n+1}}{(q^2; q^2)_n} \quad (28)$$

$$\frac{1}{(q; q^8)_{\infty} (q^5; q^8)_{\infty} (q^6; q^8)_{\infty}} = \sum_{n=0}^{\infty} \frac{q^{n^2+n} (-q; q^2)_{n+1}}{(q^2; q^2)_n} \quad (29)$$

$$\frac{(q^{10}; q^{20})_{\infty}}{(q; q^{20})_{\infty} (q^5; q^{20})_{\infty} (q^8; q^{20})_{\infty} (q^9; q^{20})_{\infty} (q^{11}; q^{20})_{\infty} (q^{12}; q^{20})_{\infty} (q^{15}; q^{20})_{\infty} (q^{19}; q^{20})_{\infty}} \\ = \sum_{n=0}^{\infty} \frac{q^{3n^2+2n} (-q; q^2)_{n+1}}{(q^2; q^2)_{2n+1}} \quad (30)$$

$$\frac{(q^2; q^{12})_\infty}{(q; q^{12})_\infty (q^3; q^{12})_\infty (q^7; q^{12})_\infty (q^9; q^{12})_\infty} = \sum_{n=0}^{\infty} \frac{q^{(3n^2+3n)/2} (-q; q^3)_{n+1}}{(q^3; q^3)_n} \quad (31)$$

$$\frac{1}{(q; q^4)_\infty (q^2; q^4)_\infty (q^3; q^4)_\infty} = \sum_{n=0}^{\infty} \frac{q^{(n^2+n)/2} (-q^2; q)_{n+1}}{(q; q)_n} \quad (32)$$

$$\frac{1}{(q; q^{20})_\infty (q^3; q^{20})_\infty (q^4; q^{20})_\infty (q^5; q^{20})_\infty (q^7; q^{20})_\infty (q^9; q^{20})_\infty (q^{11}; q^{20})_\infty (q^{13}; q^{20})_\infty (q^{15}; q^{20})_\infty (q^{16}; q^{20})_\infty (q^{17}; q^{20})_\infty (q^{19}; q^{20})_\infty} = \sum_{n=0}^{\infty} \frac{q^{n^2} (-q; q)_{2n}}{(q^2; q^2)_{2n}} \quad (33)$$

$$\frac{1}{(q; q^2)_\infty} = \sum_{n=0}^{\infty} \frac{q^{2n^2+n} (-q; q)_{2n+1}}{(q^2; q^2)_{2n+1}} \quad (34)$$

$$\frac{1}{(q; q^{16})_\infty (q^4; q^{16})_\infty (q^6; q^{16})_\infty (q^7; q^{16})_\infty (q^9; q^{16})_\infty (q^{10}; q^{16})_\infty (q^{12}; q^{16})_\infty (q^{15}; q^{16})_\infty} = \sum_{n=0}^{\infty} \frac{q^{2n^2+2n} (-q; q)_{2n+1}}{(q^2; q^2)_{2n+1}} \quad (35)$$

$$\frac{1}{(q; q^{20})_\infty (q^2; q^{20})_\infty (q^5; q^{20})_\infty (q^6; q^{20})_\infty (q^8; q^{20})_\infty (q^9; q^{20})_\infty (q^{11}; q^{20})_\infty (q^{12}; q^{20})_\infty (q^{14}; q^{20})_\infty (q^{15}; q^{20})_\infty (q^{18}; q^{20})_\infty (q^{19}; q^{20})_\infty} = \sum_{n=0}^{\infty} \frac{q^{n^2+n} (-q; q)_{2n+1}}{(q^2; q^2)_{2n+1}} \quad (36)$$

$$\frac{1}{(q; q^{20})_\infty (q^3; q^{20})_\infty (q^5; q^{20})_\infty (q^7; q^{20})_\infty (q^8; q^{20})_\infty (q^9; q^{20})_\infty (q^{11}; q^{20})_\infty (q^{12}; q^{20})_\infty (q^{13}; q^{20})_\infty (q^{15}; q^{20})_\infty (q^{17}; q^{20})_\infty (q^{19}; q^{20})_\infty} = \sum_{n=0}^{\infty} \frac{q^{n^2+2n} (-q; q)_{2n+1}}{(q^2; q^2)_{2n+1}} \quad (37)$$

$$\frac{(q^2; q^{12})_\infty (q^{10}; q^{12})_\infty}{(q; q^{12})_\infty (q^3; q^{12})_\infty^2 (q^5; q^{12})_\infty (q^7; q^{12})_\infty (q^9; q^{12})_\infty^2 (q^{11}; q^{12})_\infty} = \sum_{n=0}^{\infty} \frac{q^{(3n^2+3n)/2} (-q; q)_{3n+1}}{(q^3; q^3)_{2n+1}} \quad (38)$$